@@ -1,0 +1,10 @@
+/-
+`argraw` meets its specification, given `myproc`.
+-/
+import Xv6.ProofArgraw
+
+namespace Xv6
+
+theorem Argraw (MP : MYPROC) : ARGRAW := argraw_proof MP
+
+end Xv6
